src/Std/Data/DHashMap/Basic.lean
@@ -76,6 +76,8 @@ structure Equiv (m₁ m₂ : DHashMap α β) where
   /-- Internal implementation detail of the hash map -/
   inner : m₁.1.Equiv m₂.1
 
+@[inherit_doc] scoped infixl:50 " ~m " => Equiv
+
 @[inline, inherit_doc Raw.insert] def insert (m : DHashMap α β) (a : α)
     (b : β a) : DHashMap α β :=
   ⟨Raw₀.insert ⟨m.1, m.2.size_buckets_pos⟩ a b, .insert₀ m.2⟩
